lakefile.lean
@@ -25,5 +25,5 @@ lean_exe srcheck {
   root := `Experiments.SR.Main
 }
 
-require mathlib from git "https://github.com/leanprover-community/mathlib4" @ "v4.18.0"
-require Cli from git "https://github.com/leanprover/lean4-cli" @ "v4.18.0"
+require mathlib from git "https://github.com/leanprover-community/mathlib4" @ "v4.21.0"
+require Cli from git "https://github.com/leanprover/lean4-cli" @ "v4.21.0"
